DependentComputability/Tactic/ConvertToNew.lean
@@ -1,4 +1,5 @@
 import DependentComputability.SortExtra
+import DependentComputability.Tactic.Delab
 
 open Lean Meta
 @[inline]
@@ -210,6 +211,44 @@ def convertStructCtorType (ind : Name) (e : Expr) (ctorType : Expr) (baseMap : F
         let res ← mkForallFVars newVars newIndApp
         return res.replaceFVars baseVars (Array.ofFn fun i : Fin baseVars.size => .proj ind i e)
 
+def mkNewStructRecursor (rec : RecursorVal) (ctor : ConstructorVal) : MetaM Unit := do
+  let levels := rec.levelParams.map Level.param
+  let newRecType := mkExtraApp (← conversionStepNew rec.type) (.const rec.name levels)
+  forallTelescope rec.type fun vars _body => do
+  withNonBaseVars vars convertTypeSimpleNew fun newVars _baseMap => do
+    let params := vars.take rec.numParams
+    let newMotive := newVars[rec.numParams]!
+    let minor := vars[rec.numParams + 1]!
+    let newMinor := newVars[rec.numParams + 1]!
+    let major := vars[rec.numParams + 2]!
+    let newMajor := newVars[rec.numParams + 2]!
+    let recApp := mkAppN (.const rec.name levels) vars
+    let newResultType := mkExtraApp (mkApp2 newMotive major newMajor) recApp
+    let ourMotive ← mkLambdaFVars #[major] (← mkForallFVars #[newMajor] newResultType)
+    let lvl ← getLevel (← inferType major)
+    let ourRecApp := .const rec.name (levels.modifyHead lvl.imax)
+    let ourRecApp := mkAppN ourRecApp params
+    let ourRecApp := ourRecApp.app ourMotive
+    let ourMinor ← forallTelescope (← inferType minor) fun fields body => do
+      let .app _motive motiveArg := body | throwError "internal error"
+      let newMajorType := (← inferType newMajor).replaceFVar major motiveArg
+      withLocalDeclD `t newMajorType fun newMajor => do
+        let newFields := Array.ofFn fun n : Fin fields.size =>
+          .proj (mkNewInductName ctor.induct) n newMajor
+        let value := mkAppN newMinor (fields.interleave newFields)
+        mkLambdaFVars (fields.push newMajor) value
+    let ourRecApp := ourRecApp.app ourMinor
+    let vars := (vars.interleave newVars).take ((vars.size - 1) * 2)
+    let value ← mkLambdaFVars vars ourRecApp
+    addDecl <| .defnDecl {
+      name := mkNewName rec.name
+      levelParams := rec.levelParams
+      type := newRecType
+      value := value
+      hints := .abbrev
+      safety := .safe
+    }
+
 mutual
 
 partial def convertStructureType (info : InductiveVal) : MetaM Unit := do
@@ -265,10 +304,12 @@ partial def convertStructureType (info : InductiveVal) : MetaM Unit := do
     hints := .abbrev
     safety := .safe
   }
+  let rec ← getConstInfoRec (mkRecName info.name)
+  mkNewStructRecursor rec ctor
 
 partial def toNewInductiveType (info : InductiveVal) : MetaM InductiveType := do
   if info.isNested then
-    throwError "nested not supported"
+    throwError "nested {info.name} not supported"
   let ind := info.name
   let all := info.all
   let lparams' := info.levelParams.map Level.param
@@ -330,93 +371,100 @@ partial def convertInductToNew (val : InductiveVal) : MetaM Unit := do
     addNewRecursor ind info recNames
 
 partial def recConvertToNew (nm : Name) : CoreM Unit := do
-  if (← getEnv).contains (`New ++ nm) then
-    return
-  let info ← getConstInfo nm
-  match info with
-  | .defnInfo val =>
-    let type := val.type
-    let value := val.value
-    Meta.MetaM.run' do
-      let consts := type.getUsedConstantsAsSet.merge value.getUsedConstantsAsSet
-      for c in consts do
-        recConvertToNew c
-      let newType ← conversionStepNew type
-      let newValue ← conversionStepNew value
-      let newType' : Expr := .app (.proj ``SortExtra 0 newType)
-        (.const val.name (val.levelParams.map Level.param))
-      Lean.addDecl <| .defnDecl {
-        name := `New ++ nm
-        levelParams := val.levelParams
-        type := newType'
-        value := newValue
-        hints := val.hints
-        safety := val.safety
-      }
-  | .thmInfo val =>
-    let type := val.type
-    for c in type.getUsedConstantsAsSet do
-      recConvertToNew c
-    Meta.MetaM.run' do
-      let newType ← conversionStepNew type
-      let const := .const val.name (val.levelParams.map Level.param)
-      let newType' : Expr := .app (.proj ``SortExtra 0 newType) const
-      -- attempt transfer
-      let instType := mkApp2 (.const ``NonemptyExtra [levelZero]) type newType
-      let mut newValue := default
-      if let some inst ← synthInstance? instType then
-        newValue := mkApp4 (.const ``NonemptyExtra.transfer []) type newType inst const
-      else
-        let value := val.value
-        let consts := value.getUsedConstantsAsSet
+  try
+    if (← getEnv).contains (mkNewName nm) then
+      return
+    let info ← getConstInfo nm
+    match info with
+    | .defnInfo val =>
+      let type := val.type
+      let value := val.value
+      Meta.MetaM.run' do
+        let consts := type.getUsedConstantsAsSet.merge value.getUsedConstantsAsSet
         for c in consts do
           recConvertToNew c
-        newValue ← conversionStepNew value
-      Lean.addDecl <| .thmDecl {
-        name := `New ++ nm
-        levelParams := val.levelParams
-        type := newType'
-        value := newValue
-      }
-  | .inductInfo val => (convertInductToNew val).run'
-  | .ctorInfo val => recConvertToNew val.induct
-  | _ => throwError "unhandled const info {.ofConstName nm}"
+        let newType ← conversionStepNew type
+        let newValue ← conversionStepNew value
+        let newType' : Expr := .app (.proj ``SortExtra 0 newType)
+          (.const val.name (val.levelParams.map Level.param))
+        Lean.addDecl <| .defnDecl {
+          name := mkNewName nm
+          levelParams := val.levelParams
+          type := newType'
+          value := newValue
+          hints := val.hints
+          safety := val.safety
+        }
+    | .thmInfo val =>
+      let type := val.type
+      for c in type.getUsedConstantsAsSet do
+        recConvertToNew c
+      Meta.MetaM.run' do
+        let newType ← conversionStepNew type
+        let const := .const val.name (val.levelParams.map Level.param)
+        let newType' : Expr := .app (.proj ``SortExtra 0 newType) const
+        -- attempt transfer
+        let instType := mkApp2 (.const ``NonemptyExtra [levelZero]) type newType
+        let mut newValue := default
+        if let some inst ← synthInstance? instType then
+          newValue := mkApp4 (.const ``NonemptyExtra.transfer []) type newType inst const
+        else
+          let value := val.value
+          let consts := value.getUsedConstantsAsSet
+          for c in consts do
+            recConvertToNew c
+          newValue ← conversionStepNew value
+        Lean.addDecl <| .thmDecl {
+          name := mkNewName nm
+          levelParams := val.levelParams
+          type := newType'
+          value := newValue
+        }
+    | .inductInfo val => (convertInductToNew val).run'
+    | .ctorInfo val => recConvertToNew val.induct
+    | _ => throwError "unhandled const info {.ofConstName nm}"
+  catch ex =>
+    let msg := ex.toMessageData ++ m!"\nin {.ofConstName nm}"
+    throwError msg
 
 end
 
 elab "convert_to_new " id:ident : command => do
   Lean.Elab.Command.liftCoreM do
     let name ← Lean.Elab.realizeGlobalConstNoOverloadWithInfo id
-    recConvertToNew name
+    if (← getEnv).contains (mkNewName name) then
+      logWarning m!"{name} has already been translated"
+    else
+      recConvertToNew name
 
-convert_to_new List
-convert_to_new Option
-convert_to_new PProd
+/-!
+Essentials
+-/
 
 noncomputable opaque uniqueChoice (h : Nonempty α) : Squash α :=
   .mk (Classical.choice h)
 
 namespace New
 
-protected def Nat : convert_to_new_type% Nat :=
+protected def Nat : new_type% Nat :=
   .mk (fun _ => Unit) (fun {n} _ m => n = m) (IsPropEncodingTrivial.univElim.{0} _)
 
-protected def Nat.zero : convert_to_new_type% @Nat.zero := ()
-protected def Nat.succ : convert_to_new_type% @Nat.succ := fun _ _ => ()
+protected def Nat.zero : new_type% @Nat.zero := ()
+protected def Nat.succ : new_type% @Nat.succ := fun _ _ => ()
 
-protected def Nat.rec.{u} : convert_to_new_type% @Nat.rec.{u} :=
+protected def Nat.rec.{u} : new_type% @Nat.rec.{u} :=
   fun {_} _ {_} zero {_} succ {t_base} _ => t_base.rec zero fun _ ih => succ () ih
 
-protected def PUnit.{u} : convert_to_new_type% @PUnit.{u} :=
+protected def PUnit.{u} : new_type% @PUnit.{u} :=
   .mk (fun _ => PUnit.{u}) (TrivialEncoding _) (.trivialEncoding _)
 
-protected def PUnit.unit.{u} : convert_to_new_type% @PUnit.unit.{u} :=
+protected def PUnit.unit.{u} : new_type% @PUnit.unit.{u} :=
   @_root_.PUnit.unit.{u}
 
 convert_to_new Iff
 convert_to_new Eq
 
-protected theorem propext : convert_to_new_type% @propext := by
+protected theorem propext : new_type% @propext := by
   intro p_base p q_base q h_base h
   dsimp only
   cases propext h_base
@@ -425,42 +473,34 @@ protected theorem propext : convert_to_new_type% @propext := by
   cases pelim.eq
   cases qelim.eq
   rcases h with ⟨hmp, hmpr⟩
-  by_cases hbase : p_base
-  · cases eq_true hbase
-    have : pty = qty := by
-      ext h
-      exact ⟨@hmp trivial, @hmpr trivial⟩
-    subst this
-    constructor
-  · cases eq_false hbase
-    have : pty = qty := by
-      ext h
-      exact h.elim
-    subst this
-    constructor
+  have : pty = qty := by
+    ext h
+    exact ⟨@hmp h, @hmpr h⟩
+  cases this
+  constructor
 
 set_option bootstrap.inductiveCheckResultingUniverse false in
 set_option genSizeOf false in
 set_option genInjectivity false in
-inductive Quot._base {α_base : Sort u} {α : convert_to_new_type% α_base}
-    {r_base : α_base → α_base → Prop} (r : convert_to_new_type% r_base) :
+inductive Quot._base {α_base : Sort u} {α : new_type% α_base}
+    {r_base : α_base → α_base → Prop} (r : new_type% r_base) :
     Quot r_base → Sort u where
   | mk {a_base : α_base} (a : α.1 a_base) : _base r (Quot.mk r_base a_base)
 
-inductive Quot._rel {α_base : Sort u} {α : convert_to_new_type% α_base}
-    {r_base : α_base → α_base → Prop} (r : convert_to_new_type% r_base) :
+inductive Quot._rel {α_base : Sort u} {α : new_type% α_base}
+    {r_base : α_base → α_base → Prop} (r : new_type% r_base) :
     (q : Quot r_base) → Quot._base r q → Quot._base r q → Prop where
   | mk {a_base : α_base} (a : α.1 a_base) {b_base : α_base} (b : α.1 b_base)
     {h_base : r_base a_base b_base} (h : (r a b).1 h_base) :
     _rel r (Quot.mk r_base b_base) (Quot.sound h_base ▸ .mk a) (.mk b)
 
-inductive Quot._encoding {α_base : Sort u} {α : convert_to_new_type% α_base}
-    {r_base : α_base → α_base → Prop} (r : convert_to_new_type% r_base) :
+inductive Quot._encoding {α_base : Sort u} {α : new_type% α_base}
+    {r_base : α_base → α_base → Prop} (r : new_type% r_base) :
     ⦃q_base : Quot r_base⦄ → (q : Quot (_rel r q_base)) → (n : ℕ) → Prop where
   | mk {a_base : α_base} {a : α.1 a_base} {n : ℕ} (h : α.2 a n) :
     @_encoding α_base α r_base r (Quot.mk r_base a_base) (Quot.mk _ (.mk a)) n
 
-protected def Quot.{u} : convert_to_new_type% @Quot.{u} := fun α_base α r_base r =>
+protected def Quot.{u} : new_type% @Quot.{u} := fun α_base α r_base r =>
   .mk (fun q => Quot (Quot._rel r q)) (Quot._encoding r) <| by
     intro hprop a_base a n
     simp only [trivialEncoding_iff]
@@ -472,15 +512,15 @@ protected def Quot.{u} : convert_to_new_type% @Quot.{u} := fun α_base α r_base
       constructor
       exact (α.3 hprop _ _).mpr .zero
 
-protected def Quot.mk.{u} : convert_to_new_type% @Quot.mk.{u} := fun _ _ _ _ _ a =>
+protected def Quot.mk.{u} : new_type% @Quot.mk.{u} := fun _ _ _ _ _ a =>
   _root_.Quot.mk _ (.mk a)
 
-protected theorem Quot.ind.{u} : convert_to_new_type% @Quot.ind.{u} := by
+protected theorem Quot.ind.{u} : new_type% @Quot.ind.{u} := by
   intro α_base α r_base r motive_base motive mk_base mk t_base t
   rcases t with ⟨@⟨t_base, t⟩⟩
   apply mk
 
-protected def Quot.lift.{u, v} : convert_to_new_type% @Quot.lift.{u, v} :=
+protected def Quot.lift.{u, v} : new_type% @Quot.lift.{u, v} :=
   fun α_base α r_base r β_base β f_base f h_base h q_base q =>
     _root_.Quot.lift (fun x : _base r q_base =>
       haveI : _root_.Quot.lift f_base h_base q_base = f_base x.1 := by
@@ -495,7 +535,7 @@ where finally
   refine (h a b hab).rec ?_
   rfl
 
-protected theorem Quot.sound.{u} : convert_to_new_type% @Quot.sound.{u} := by
+protected theorem Quot.sound.{u} : new_type% @Quot.sound.{u} := by
   intro α_base α r_base r a_base a b_base b h_base h
   dsimp only
   have sound_base := _root_.Quot.sound h_base
@@ -513,7 +553,7 @@ convert_to_new instSubsingletonSquash
 
 theorem _root_.subsingletonExtra_of_subsingleton
     {α_base : Sort u} (α : New.Sort.1 α_base)
-    {h_base : _root_.Subsingleton α_base} (h : convert_to_new_type% h_base) :
+    {h_base : _root_.Subsingleton α_base} (h : new_type% h_base) :
     SubsingletonExtra α := by
   constructor
   intro x
@@ -525,7 +565,7 @@ theorem _root_.subsingletonExtra_of_subsingleton
 instance {α_base : Sort u} (α : New.Sort.1 α_base) : SubsingletonExtra (Squash α) :=
   subsingletonExtra_of_subsingleton _ (instSubsingletonSquash α)
 
-protected noncomputable def uniqueChoice.{u} : convert_to_new_type% @uniqueChoice.{u} :=
+protected noncomputable def uniqueChoice.{u} : new_type% @uniqueChoice.{u} :=
   fun α_base α h_base h =>
     haveI : _root_.Nonempty ((a : α_base) ×' α.1 a) := by
       obtain @⟨a_base, a⟩ := h
@@ -536,7 +576,7 @@ protected noncomputable def uniqueChoice.{u} : convert_to_new_type% @uniqueChoic
 
 end New
 
-instance {α_base : Sort u} (α : convert_to_new_type% α_base) [SubsingletonExtra α]
+instance {α_base : Sort u} (α : new_type% α_base) [SubsingletonExtra α]
     {a_base : α_base} (a : α.1 a_base)
     {b_base : α_base} (b : α.1 b_base) :
     NonemptyExtra (New.Eq α a b) where
@@ -546,84 +586,348 @@ instance {α_base : Sort u} (α : convert_to_new_type% α_base) [SubsingletonExt
     constructor
     constructor
 
-instance {α_base : Sort u} (α : New.Sort.1 α_base) {β_base : α_base → Sort v}
-    (β : ⦃a_base : α_base⦄ → α.1 a_base → New.Sort.1 (β_base a_base))
-    [∀ a_base a, NonemptyExtra (@β a_base a)] :
-    NonemptyExtra (New.Forall α β) where
-  nonempty f := by
-    constructor
-    intro a_base a
-    exact Classical.choice (NonemptyExtra.nonempty (f a_base))
-
-instance {α_base : Sort u} (α : New.Sort.1 α_base) {β_base : α_base → Sort v}
-    (β : ⦃a_base : α_base⦄ → α.1 a_base → New.Sort.1 (β_base a_base))
-    [∀ a_base a, SubsingletonExtra (@β a_base a)] :
-    SubsingletonExtra (New.Forall α β) where
-  subsingleton f := by
-    constructor
-    intro a_base a
-    funext x_base x
-    apply Subsingleton.allEq
-
-instance {α_base : Type u} (α : New.Sort.1 α_base) {β_base : α_base → Type v}
-    (β : ⦃a_base : α_base⦄ → α.1 a_base → New.Sort.1 (β_base a_base))
-    [∀ a_base a, UniqueExtra (@β a_base a)] :
-    UniqueExtra (New.Forall α β) where
-  default f_base := fun {a_base} _ => UniqueExtra.default (f_base a_base)
-
 instance : UniqueExtra New.Nat where
   default _ := ()
   subsingleton _ := inferInstanceAs (Subsingleton Unit)
 
-def uniqueNatVal (n : Nat) : convert_to_new_type% n := ()
+def uniqueNatVal (n : Nat) : new_type% n := ()
 
-convert_to_new Nat.add
-convert_to_new Nat.sub
-convert_to_new Nat.mul
-convert_to_new HEq
-convert_to_new eq_of_heq
-convert_to_new And
+inductive New.Subtype._induct {α_base : Sort u} {α : new_type% α_base}
+    {p_base : α_base → Prop} (p : new_type% p_base) (t : Subtype p_base) where
+  | mk (val : α.1 t.1) (property : (p val).1 t.2)
 
-def New.And.rec.{u} : convert_to_new_type% @And.rec.{u} := by
-  intro p_base p q_base q motive_base motive intro_base intro t_base t
-  exact t_base.rec fun _ _ => intro t.1 t.2
+inductive New.Subtype._encoding {α_base : Sort u} {α : new_type% α_base}
+    {p_base : α_base → Prop} (p : new_type% p_base)
+    ⦃t_base : Subtype p_base⦄ (t : _induct p t_base) (n : ℕ) : Prop where
+  | mk (val_enc : α.2 t.1 n)
 
-convert_to_new Nat.mod
-convert_to_new Nat.div
+def New.Subtype : new_type% @Subtype.{u} := fun _ _ _ p =>
+  .mk (Subtype._induct p) (Subtype._encoding p) (.univElim _)
+
+def New.Subtype.mk : new_type% @Subtype.mk.{u} :=
+  fun _ _ _ _ _ x _ y => ⟨x, y⟩
+
+def New.Subtype.rec.{v, u} : new_type% @Subtype.rec.{v, u} :=
+  fun _ _ _ _ _ _ _ intro _ t => intro t.1 t.2
+
+@[simp]
+theorem encoding_subtype_def {α_base : Sort u} {α : new_type% α_base}
+    {p_base : α_base → Prop} {p : new_type% p_base}
+    {t_base : Subtype p_base} {t : new_type% t_base} {n : ℕ} :
+    (new% Subtype p_base).2 t n ↔ α.2 t.1 n := by
+  constructor
+  · rintro ⟨h⟩
+    exact h
+  · intro h
+    exact ⟨h⟩
+
+inductive New.List._induct {α_base : Type u} (α_extra : α_base → Type u) :
+    List α_base → Type u where
+  | nil : _induct α_extra []
+  | cons {head_base : α_base} (head : α_extra head_base)
+    {tail_base : List α_base} (tail : _induct α_extra tail_base) :
+    _induct α_extra (head_base :: tail_base)
+
+inductive New.List._encoding {α_base : Type u}
+    (α_extra : α_base → Type u) (α_enc : ⦃t_base : α_base⦄ → α_extra t_base → ℕ → Prop) :
+    ⦃l_base : List α_base⦄ → _induct α_extra l_base → ℕ → Prop where
+  | nil : _encoding α_extra α_enc .nil .zero
+  | cons {head_base : α_base} {head : α_extra head_base}
+    {head_n : ℕ} (head_enc : α_enc head head_n)
+    {tail_base : List α_base} {tail : _induct α_extra tail_base}
+    {tail_n : ℕ} (tail_enc : _encoding α_extra α_enc tail tail_n) :
+    _encoding α_extra α_enc (.cons head tail) (.succ (Nat.pair head_n tail_n))
+
+def New.List : new_type% @List.{u} :=
+  fun _ α => .mk (New.List._induct α.1) (New.List._encoding α.1 α.2)
+    (IsPropEncodingTrivial.univElim.{u + 1} _)
+
+def New.List.nil : new_type% @List.nil.{u} :=
+  fun _ α => @New.List._induct.nil _ α.1
+
+def New.List.cons : new_type% @List.cons.{u} :=
+  fun _ α => @New.List._induct.cons _ α.1
+
+noncomputable def New.List.rec.{u, v} : new_type% @List.rec.{u, v} :=
+  fun _ _ _ _ _ nil _ cons _ t => t.rec nil (fun _ _ _ ih => cons _ _ ih)
+
+set_option inductive.autoPromoteIndices false in
+inductive New.Array._induct {α_base : Type u} (α_extra : α_base → Type u)
+    (t : Array α_base) : Type u where
+  | mk (toList : New.List._induct α_extra t.1) : _induct α_extra t
+
+inductive New.Array._encoding {α_base : Type u}
+    (α_extra : α_base → Type u) (α_enc : ⦃t_base : α_base⦄ → α_extra t_base → ℕ → Prop)
+    ⦃l_base : Array α_base⦄ (l : _induct α_extra l_base) (n : ℕ) : Prop where
+  | mk (toList : New.List._encoding α_extra α_enc l.1 n)
+
+def New.Array : new_type% @Array.{u} :=
+  fun _ α => .mk (New.Array._induct α.1) (New.Array._encoding α.1 α.2)
+    (IsPropEncodingTrivial.univElim.{u + 1} _)
+
+def New.Array.mk : new_type% @Array.mk.{u} :=
+  fun _ α _ toList => @New.Array._induct.mk _ α.1 _ toList
+
+def New.Array.rec.{u, v} : new_type% @Array.rec.{u, v} :=
+  fun _ _ _ _ _ mk _ t => mk t.1
+
+convert_to_new String
+
+instance {α_base : Type u} {α : new_type% α_base} [SubsingletonExtra α] :
+    SubsingletonExtra (New.List α) where
+  subsingleton t_base := by
+    constructor
+    intro t₁ t₂
+    induction t₁ with
+    | nil => cases t₂; rfl
+    | cons head tail ih =>
+      rcases t₂ with _ | ⟨head', tail'⟩
+      cases Subsingleton.allEq head head'
+      cases ih tail'
+      rfl
+
+instance {α_base : Type u} {α : new_type% α_base} [UniqueExtra α] : UniqueExtra (New.List α) where
+  default t_base := t_base.rec .nil fun head _ ih => .cons (UniqueExtra.default head) ih
+
+instance {α_base : Type u} {α : new_type% α_base} [SubsingletonExtra α] :
+    SubsingletonExtra (New.Array α) where
+  subsingleton t_base := by
+    constructor
+    intro t₁ t₂
+    refine congrArg New.Array._induct.mk ?_
+    apply Subsingleton.allEq (α := new_type% t_base.1)
+
+instance {α_base : Type u} {α : new_type% α_base} [UniqueExtra α] : UniqueExtra (New.Array α) where
+  default t_base := t_base.rec fun a => .mk
+    (show new_type% a from UniqueExtra.default (α := New.List α) a)
+
+def nonemptyExtraOfDecidable {p_base : Prop} {p : new_type% p_base}
+    {h_base : Decidable p_base} (h : new_type% h_base) :
+    NonemptyExtra p where
+  nonempty t_base := by
+    cases h
+    · contradiction
+    · constructor; assumption
+
+instance {n_base : ℕ} {n : new_type% n_base} {m_base : ℕ} {m : new_type% m_base} :
+    NonemptyExtra (@New.Nat.le n_base n m_base m) :=
+  nonemptyExtraOfDecidable (new% Nat.decLe n_base m_base)
+
+instance {n_base : ℕ} {n : new_type% n_base} {m_base : ℕ} {m : new_type% m_base} :
+    NonemptyExtra (new% n_base ≤ m_base) := instNonemptyExtraLeLe
+
+instance {n_base : ℕ} {n : new_type% n_base} {m_base : ℕ} {m : new_type% m_base} :
+    NonemptyExtra (new% n_base < m_base) := instNonemptyExtraLeLe
+
+instance {n_base : ℕ} {n : new_type% n_base} : UniqueExtra (@New.Fin n_base n) where
+  subsingleton t_base := by
+    constructor
+    rintro ⟨⟩ ⟨⟩; rfl
+  default t_base :=
+    .mk _ _ () (NonemptyExtra.transfer (@New.Nat.le t_base.succ () n_base ()) t_base.2)
+
+instance {n_base : ℕ} {n : new_type% n_base} : UniqueExtra (@New.BitVec n_base n) where
+  subsingleton t_base := by
+    constructor
+    rintro ⟨⟨⟩⟩ ⟨⟨⟩⟩; rfl
+  default t_base := .ofFin _ _ (UniqueExtra.default (α := new% Fin (Nat.pow 2 n_base)) t_base.1)
+
+instance : UniqueExtra New.UInt8 where
+  subsingleton t_base := by
+    constructor
+    rintro ⟨⟨⟨⟩⟩⟩ ⟨⟨⟨⟩⟩⟩; rfl
+  default t_base := .ofBitVec _ (UniqueExtra.default (α := new% BitVec 8) t_base.1)
+
+instance : UniqueExtra New.UInt32 where
+  subsingleton t_base := by
+    constructor
+    rintro ⟨⟨⟨⟩⟩⟩ ⟨⟨⟨⟩⟩⟩; rfl
+  default t_base := .ofBitVec _ (UniqueExtra.default (α := new% BitVec 32) t_base.1)
+
+convert_to_new inferInstance
+convert_to_new instDecidableOr
+convert_to_new instDecidableAnd
+
+instance {n_base : UInt32} (n : new_type% n_base) :
+    NonemptyExtra (New.UInt32.isValidChar n) :=
+  nonemptyExtraOfDecidable (new% (inferInstance : Decidable (UInt32.isValidChar n_base)))
+
+instance : UniqueExtra New.Char where
+  subsingleton t_base := by
+    constructor
+    rintro ⟨⟨⟨⟨⟩⟩⟩⟩ ⟨⟨⟨⟩⟩⟩; rfl
+  default t_base := .mk _ (UniqueExtra.default (α := New.UInt32) t_base.1)
+    (NonemptyExtra.transfer (@New.UInt32.isValidChar t_base.1 _) _)
+
+instance : UniqueExtra New.ByteArray where
+  subsingleton t_base := by
+    constructor
+    rintro ⟨a⟩ ⟨b⟩
+    cases Subsingleton.allEq a b; rfl
+  default t_base := t_base.rec fun a => .mk _
+    (show new_type% a from UniqueExtra.default (α := New.Array New.UInt8) a)
+
+instance {b_base : ByteArray} (b : new_type% b_base) :
+    NonemptyExtra (New.ByteArray.IsValidUTF8 b) where
+  nonempty t_base := by
+    rcases t_base with ⟨l, hl⟩
+    constructor
+    refine @New.ByteArray.IsValidUTF8._induct.intro _ _ l ?_ hl ?_
+    · with_reducible exact UniqueExtra.default _
+    · with_reducible exact NonemptyExtra.transfer _ _
+
+instance : UniqueExtra New.String where
+  subsingleton t_base := by
+    constructor
+    rintro ⟨a⟩ ⟨b⟩
+    cases Subsingleton.allEq a b; rfl
+  default t_base := .ofByteArray _ (UniqueExtra.default (α := New.ByteArray) _)
+    (NonemptyExtra.transfer (@New.ByteArray.IsValidUTF8 t_base.1 _) _)
+
+noncomputable def uniqueStrVal (s : String) : new_type% s :=
+  UniqueExtra.default (α := new% String) s
+
+convert_to_new SourceInfo
+convert_to_new SyntaxNodeKind
+convert_to_new Syntax.Preresolved
+
+inductive New.Lean.Syntax._induct : Lean.Syntax → Type where
+  | missing : _induct .missing
+  | node
+    {info_base : _root_.Lean.SourceInfo} (info : new_type% info_base)
+    {kind_base : _root_.Lean.SyntaxNodeKind} (kind : new_type% kind_base)
+    {args_base : _root_.Array _root_.Lean.Syntax}
+    (args : @New.List._induct Lean.Syntax _induct args_base.1) :
+    _induct (.node info_base kind_base args_base)
+  | atom {info_base : _root_.Lean.SourceInfo} (info : new_type% info_base)
+    {val_base : _root_.String} (val : new_type% val_base) : _induct (.atom info_base val_base)
+  | ident {info_base : _root_.Lean.SourceInfo} (info : new_type% info_base)
+    {rawVal_base : _root_.Substring.Raw} (rawVal : new_type% rawVal_base)
+    {val_base : _root_.Lean.Name} (val : new_type% val_base)
+    {preresolved_base : _root_.List _root_.Lean.Syntax.Preresolved}
+    (preresolved : new_type% preresolved_base) :
+    _induct (.ident info_base rawVal_base val_base preresolved_base)
+
+inductive New.Lean.Syntax._encoding : ⦃t_base : Lean.Syntax⦄ → _induct t_base → ℕ → Prop where
+  | missing : _encoding .missing 0
+  | node
+    {info_base : _root_.Lean.SourceInfo} {info : new_type% info_base}
+    {info_n : ℕ} (info_enc : New.Lean.SourceInfo.2 info info_n)
+    {kind_base : _root_.Lean.SyntaxNodeKind} {kind : new_type% kind_base}
+    {kind_n : ℕ} (kind_enc : New.Lean.SyntaxNodeKind.2 kind kind_n)
+    {args_base : _root_.Array _root_.Lean.Syntax}
+    {args : @New.List._induct Lean.Syntax _induct args_base.1}
+    {args_n : ℕ} (args_enc : New.List._encoding _induct _encoding args args_n) :
+    _encoding (.node info kind args) (Nat.pair info_n (Nat.pair kind_n args_n) * 3 + 1)
+  | atom {info_base : _root_.Lean.SourceInfo} {info : new_type% info_base}
+    {info_n : ℕ} (info_enc : New.Lean.SourceInfo.2 info info_n)
+    {val_base : _root_.String} {val : new_type% val_base}
+    {val_n : ℕ} (val_enc : New.String.2 val val_n) :
+    _encoding (.atom info val) (Nat.pair info_n val_n * 3 + 2)
+  | ident  {info_base : _root_.Lean.SourceInfo} {info : new_type% info_base}
+    {info_n : ℕ} (info_enc : New.Lean.SourceInfo.2 info info_n)
+    {rawVal_base : _root_.Substring.Raw} {rawVal : new_type% rawVal_base}
+    {rawVal_n : ℕ} (rawVal_enc : New.Substring.Raw.2 rawVal rawVal_n)
+    {val_base : _root_.Lean.Name} (val : new_type% val_base)
+    {val_n : ℕ} (val_enc : New.Lean.Name.2 val val_n)
+    {preresolved_base : _root_.List _root_.Lean.Syntax.Preresolved}
+    (preresolved : new_type% preresolved_base)
+    {preresolved_n : ℕ}
+    (preresolved_enc : (List Syntax.Preresolved).2 preresolved preresolved_n) :
+    _encoding (.ident info rawVal val preresolved)
+      (Nat.pair info_n (Nat.pair rawVal_n (Nat.pair val_n preresolved_n)) * 3 + 3)
+
+def New.Lean.Syntax : new_type% Lean.Syntax :=
+  .mk Syntax._induct Syntax._encoding (IsPropEncodingTrivial.univElim.{1} _)
+
+def New.Lean.Syntax.missing : new_type% Lean.Syntax.missing := @_induct.missing
+def New.Lean.Syntax.atom : new_type% Lean.Syntax.atom := @_induct.atom
+def New.Lean.Syntax.ident : new_type% Lean.Syntax.ident := @_induct.ident
+def New.Lean.Syntax.node : new_type% Lean.Syntax.node :=
+  fun _ info _ kind _ args => _induct.node info kind args.1
+
+noncomputable def New.Lean.Syntax.rec : new_type% @Lean.Syntax.rec.{u} :=
+  fun motive_1_base motive_1 motive_2_base _ motive_3_base motive_3
+      missing_base missing node_base node atom_base atom ident_base ident
+      mk_base mk nil_base nil cons_base cons t_base t =>
+    @Syntax._induct.rec (fun t_base t => (motive_1 t).1
+        (@_root_.Lean.Syntax.rec motive_1_base motive_2_base motive_3_base
+          missing_base node_base atom_base ident_base mk_base nil_base cons_base t_base))
+      (fun t_base t => (motive_3 t).1
+        (@_root_.Lean.Syntax.rec_2 motive_1_base motive_2_base motive_3_base
+          missing_base node_base atom_base ident_base mk_base nil_base cons_base t_base))
+      missing
+      (fun _ _ _ _ _ ih => node _ _ _ (mk _ ih))
+      @atom @ident @nil
+      (fun _ _ _ head_ih tail_ih => cons _ _ head_ih tail_ih)
+      t_base t
+
+convert_to_new Prod
+
+instance {α_base : Type u} (α : new_type% α_base)
+    {β_base : Type v} (β : new_type% β_base)
+    [SubsingletonExtra α] [SubsingletonExtra β] :
+    SubsingletonExtra (New.Prod α β) where
+  subsingleton t_base := by
+    constructor
+    rintro ⟨a, b⟩ ⟨a', b'⟩
+    cases Subsingleton.allEq a a'
+    cases Subsingleton.allEq b b'
+    rfl
+
 convert_to_new Nat.mul_add_lt_mul_of_lt_of_lt
 convert_to_new List.attach
+convert_to_new Array.attach
 convert_to_new List.mapM
 convert_to_new List.zip_eq_zip_take_min
 convert_to_new not_exists
 convert_to_new List.cons.injEq
-convert_to_new And
-convert_to_new congrArg
-convert_to_new congrFun
-convert_to_new congr
-convert_to_new Eq.trans
-convert_to_new Eq.symm
 convert_to_new eq_comm
-convert_to_new eq_true
 convert_to_new eq_false
-convert_to_new Or
 convert_to_new Part
 
-def New.Middle : convert_to_new_type% _root_.True :=
+inductive Middle : Prop where
+  | intro
+
+instance : Decidable Middle := .isTrue .intro
+
+def New.Middle : new_type% _root_.Middle :=
   .mk (fun _ => _root_.False) (TrivialEncoding _) (.trivialEncoding _)
 
-theorem not_em : ¬ convert_to_new_type% Classical.em := by
+theorem almostEm (p : Prop) : p ∨ (p ↔ Middle) ∨ ¬p := by
+  obtain h | h := Classical.em p
+  · exact .inl h
+  · exact .inr (.inr h)
+
+theorem New.almostEm : new_type% almostEm := by
+  intro p_base p
+  by_cases h : p_base
+  · by_cases h' : p.1 h
+    · exact .inl h'
+    · have iff := iff_of_true h Middle.intro
+      refine @New.Or._induct.inr _ _ _ _ (.inl iff) ?_
+      refine @New.Or._induct.inl _ _ _ _ iff ?_
+      constructor
+      · intro _ _; contradiction
+      · intro _ _; contradiction
+  · refine @New.Or._induct.inr _ _ _ _ (.inr h) ?_
+    refine @New.Or._induct.inr _ _ _ _ h ?_
+    intro h'
+    contradiction
+
+theorem not_em : ¬ new_type% Classical.em := by
   intro h
-  cases @h True New.Middle
+  cases @h Middle New.Middle
   · contradiction
   · contradiction
 
-theorem not_em' : ¬ ∃ h : type_of% Classical.em, convert_to_new_type% h := by
+theorem not_em' : ¬ ∃ h : type_of% Classical.em, new_type% h := by
   intro ⟨_, h⟩
-  cases @h True New.Middle
+  cases @h Middle New.Middle
   · contradiction
   · contradiction
 
-theorem not_not_em' : ¬ ∃ h : ¬(type_of% Classical.em), convert_to_new_type% h := by
+theorem not_not_em' : ¬ ∃ h : ¬(type_of% Classical.em), new_type% h := by
   intro ⟨h, _⟩
   simp at h
 
@@ -636,9 +940,35 @@ def splitRight (p : ℕ → Prop) : ℕ → Prop :=
 def split (p : ℕ → ℕ → Prop) : ℕ → Prop :=
   Nat.unpaired p
 
-inductive New.Prod._encodes {α_base : Type u} {α : convert_to_new_type% α_base}
-    {β_base : Type v} {β : convert_to_new_type% β_base} :
+inductive New.Prod._encodes {α_base : Type u} {α : new_type% α_base}
+    {β_base : Type v} {β : new_type% β_base} :
     {x_base : α_base × β_base} → (x : New.Prod._induct α β x_base) → Nat → Prop where
   | mk {fst_base : α_base} {fst : α.1 fst_base} {fst_num : ℕ} (fst_encodes : α.2 fst fst_num)
        {snd_base : β_base} {snd : β.1 snd_base} {snd_num : ℕ} (snd_encodes : β.2 snd snd_num) :
        _encodes (New.Prod.mk α β fst snd) (Nat.pair fst_num snd_num)
+
+convert_to_new LinearOrder
+convert_to_new LinearOrder.toPartialOrder
+convert_to_new PFun
+convert_to_new Part.instMembership
+convert_to_new Nat.lt_trichotomy
+
+lemma Nat.rfindX._proof_1_alt : type_of% @Nat.rfindX._proof_1 := by
+  intro p H m al
+  rcases H with ⟨n, h₁, h₂⟩
+  rcases Nat.lt_trichotomy m n with (h₃ | h₃ | h₃)
+  · exact h₂ _ h₃
+  · rw [h₃]
+    exact h₁.fst
+  · injection Part.mem_unique h₁ (al _ h₃)
+
+convert_to_new Nat.rfindX._proof_1_alt
+
+lemma New.Nat.rfindX._proof_1 : new_type% @Nat.rfindX._proof_1 :=
+  @New.Nat.rfindX._proof_1_alt
+
+convert_to_new New.Sort
+convert_to_new New.Forall
+convert_to_new Quot.rec
+convert_to_new New.Nat
+convert_to_new New.Nat.add
