DependentComputability/Tactic/Computability.lean
@@ -1,8 +1,8 @@
 import DependentComputability.Tactic.NewDPrimStep
+import DependentComputability.Tactic.OtherDPrimStep
 import DependentComputability.Tactic.ConvertToNew
 import DependentComputability.Tactic.Delab
-
-convert_to_new Acc
+import DependentComputability.Tactic.LetNew
 
 open scoped Delab
 
@@ -50,82 +50,144 @@ private theorem ycomb_part (thing : Code) : Nat.Partrec (ycomb thing) := by
     refine .comp .encode ?_
     exact Code.primrec₂_curry.to_comp.comp (.const _) (.comp .fst .unpair)
 
-/-open Nat.Partrec (Code) in
-theorem dcomputable_reassoc {α : Sort u} {β : α → Sort v} {γ : (a : α) ×' β a → Sort w}
-    {δ : (x : (a : α) ×' β a) ×' γ x → Sort w'}
-    [EncodingRelation α] [∀ x, EncodingRelation (β x)] [∀ x, EncodingRelation (γ x)]
-    [∀ x, EncodingRelation (δ x)]
-    (f : (x : (x : (a : α) ×' β a) ×' γ x) → δ x) :
-    DComputable f ↔ DComputable fun x : (a : α) ×' (b : β a) ×' γ ⟨a, b⟩ =>
-      f ⟨⟨x.1, x.2.1⟩, x.2.2⟩ := by
-  constructor
-  · intro hf
-    refine DComputable.comp hf (DPrimrec.dcomputable ?_)
-    dprim_tac
-  · intro hf
-    refine DComputable.comp
-      (g := fun x : (x : (a : α) ×' β a) ×' γ x => ⟨x.1.1, x.1.2, x.2⟩) hf ?_
-    refine DPrimrec.dcomputable ?_
-    dprim_tac-/
+attribute [dprim] New.PSigma.fst.computable New.PSigma.snd.computable New.PSigma.mk.computable
+  New.PSigma.fst.primrec New.PSigma.snd.primrec New.PSigma.mk.primrec
 
-/-open Nat.Partrec Denumerable in
-theorem New.Acc.rec.computable.{c, v, u}
+attribute [other_dprim] PSigma.fst.dcomp PSigma.snd.dcomp PSigma.mk.dcomp
+  PSigma.fst.dprim PSigma.snd.dprim PSigma.mk.dprim
+
+@[dprim]
+theorem _root_.New.Subtype.val.computable.{c, u} {ctx_base : Sort c} {ctx : new_type% ctx_base}
+    {α_base : ctx_base → Sort u} {α : new_type% α_base}
+    {p_base : (c : ctx_base) → α_base c → Prop} {p : new_type% p_base}
+    {self_base : (c : ctx_base) → Subtype (p_base c)} {self : new_type% self_base}
+    (self_comp : DComputable (new% self_base)) :
+    DComputable (new% fun c => (self_base c).val) := by
+  obtain ⟨g, hg, hg'⟩ := self_comp
+  use g, hg
+  simpa using hg'
+
+@[dprim]
+theorem _root_.New.Subtype.mk.computable.{c, u} {ctx_base : Sort c} {ctx : new_type% ctx_base}
+    {α_base : ctx_base → Sort u} {α : new_type% α_base}
+    {p_base : (c : ctx_base) → α_base c → Prop} {p : new_type% p_base}
+    {val_base : (c : ctx_base) → α_base c} {val : new_type% val_base}
+    (val_comp : DComputable (new% val_base))
+    {property_base : (c : ctx_base) → p_base c (val_base c)}
+    (property : new_type% property_base) :
+    DComputable (new% fun c => Subtype.mk (val_base c) (property_base c)) := by
+  obtain ⟨g, hg, hg'⟩ := val_comp
+  use g, hg
+  simpa using hg'
+
+section
+
+set_option linter.unusedVariables.funArgs false
+
+@[other_dprim]
+lemma Subtype.mk.dprim {ctx : Sort u} {α : ctx → Sort v} {β : (c : ctx) → α c → Prop}
+    {f : (c : ctx) → α c} (hf : DComp f) {g : (c : ctx) → β c (f c)} :
+    DComp (fun c => Subtype.mk (f c) (g c)) := .unsafeIntro
+
+@[other_dprim]
+lemma Subtype.val.dprim {ctx : Sort u} {α : ctx → Sort v} {β : (c : ctx) → α c → Prop}
+    {f : (c : ctx) → Subtype (β c)} (hf : DComp f) :
+    DComp (fun c => (f c).1) := .unsafeIntro
+
+@[other_dprim]
+lemma Subtype.mk.dcomp {ctx : Sort u} {α : ctx → Sort v} {β : (c : ctx) → α c → Prop}
+    {f : (c : ctx) → α c} (hf : DComp f) {g : (c : ctx) → β c (f c)} :
+    DComp (fun c => Subtype.mk (f c) (g c)) := .unsafeIntro
+
+@[other_dprim]
+lemma Subtype.val.dcomp {ctx : Sort u} {α : ctx → Sort v} {β : (c : ctx) → α c → Prop}
+    {f : (c : ctx) → Subtype (β c)} (hf : DComp f) :
+    DComp (fun c => (f c).1) := .unsafeIntro
+
+lemma _root_.New.Subtype.mk.dprim.{u, v} : new_type% @Subtype.mk.dprim.{u, v} :=
+  fun _ _ _ _ _ _ _ _ _ hf _ _ => New.Subtype.mk.computable hf _
+lemma _root_.New.Subtype.val.dprim.{u, v} : new_type% @Subtype.val.dprim.{u, v} :=
+  fun _ _ _ _ _ _ _ _ _ hf => New.Subtype.val.computable hf
+lemma _root_.New.Subtype.mk.dcomp.{u, v} : new_type% @Subtype.mk.dcomp.{u, v} :=
+  fun _ _ _ _ _ _ _ _ _ hf _ _ => New.Subtype.mk.computable hf _
+lemma _root_.New.Subtype.val.dcomp.{u, v} : new_type% @Subtype.val.dcomp.{u, v} :=
+  fun _ _ _ _ _ _ _ _ _ hf => New.Subtype.val.computable hf
+
+end
+
+convert_to_new Subtype.property
+
+open Nat.Partrec Denumerable in
+open Lean Elab Tactic in
+theorem _root_.New.Acc.rec.computable.{c, v, u}
     {ctx_base : Sort c}
-    {ctx : convert_to_new_type% ctx_base}
+    {ctx : new_type% ctx_base}
     {α_base : ctx_base → Sort u}
-    {α : convert_to_new_type% α_base}
+    {α : new_type% α_base}
     {r_base : (c : ctx_base) → α_base c → α_base c → Prop}
-    {r : convert_to_new_type% r_base}
-    {motive_base : (c : ctx_base) → (a : α_base c) → _root_.Acc (r_base c) a → Sort v}
-    {motive : convert_to_new_type% motive_base}
+    {r : new_type% r_base}
+    {motive_base : (c : ctx_base) → (a : α_base c) → Acc (r_base c) a → Sort v}
+    {motive : new_type% motive_base}
     {intro_base : (c : ctx_base) → (a : α_base c) →
-        (h : ∀ b, r_base c b a → _root_.Acc (r_base c) b) →
-      (ih : ∀ b hb, motive_base c b (h b hb)) → motive_base c a (_root_.Acc.intro a h)}
-    {intro : convert_to_new_type% intro_base}
-    (intro_comp : DComputable (convert_to_new% intro_base))
+        (h : ∀ b, r_base c b a → Acc (r_base c) b) →
+      (ih : ∀ b hb, motive_base c b (h b hb)) → motive_base c a (Acc.intro a h)}
+    {intro : new_type% intro_base}
+    (intro_comp : DComputable (new% intro_base))
     {a_base : (c : ctx_base) → α_base c}
-    {a : convert_to_new_type% a_base}
-    (a_comp : DComputable (convert_to_new% a_base))
-    {t_base : (c : ctx_base) → _root_.Acc (r_base c) (a_base c)}
-    {t : convert_to_new_type% t_base} :
-    DComputable (convert_to_new% fun c => @_root_.Acc.rec
+    {a : new_type% a_base}
+    (a_comp : DComputable (new% a_base))
+    {t_base : (c : ctx_base) → Acc (r_base c) (a_base c)}
+    {t : new_type% t_base} :
+    DComputable (new% fun c => @Acc.rec
       (α_base c) (r_base c) (motive_base c) (intro_base c) (a_base c) (t_base c)) := by
   by_cases hprop : IsProp.{imax (max (max 1 u) (imax (max 1 u) v)) v}
   · exact .of_isProp @(isProp_of_isProp_imax.{max (max 1 u) (imax (max 1 u) v), v} hprop)
   by_cases hprop : IsProp.{imax (max 1 u) v}
   · exact .of_isProp @(isProp_of_isProp_imax.{max 1 u, v} hprop)
-  /-have : DComputable (fun c : ctx =>
-      fun x :
-        (a : { a : α c // ∀ b, r c b a → Acc (r c) b }) ×'
-          (∀ b : { b // r c b a }, motive c b (a.2 b b.2)) =>
-          intro c x.1.1 x.1.2 fun b hb => x.2 ⟨b, hb⟩) := by
-    simp only [dcomputable_curry, dcomputable_reassoc] at hintro ⊢
-    let ty := (c : ctx) ×' (a : { a : α c // ∀ b, r c b a → Acc (r c) b }) ×'
-      (∀ b : { b // r c b a }, motive c b (a.2 b b.2))
-    refine DComputable.comp
-      (g := fun a : ty => ⟨a.1, a.2.1.1, a.2.1.2, fun b hb => a.2.2 ⟨b, hb⟩⟩) hintro ?_
-    dprim_tac-/
+  have_new this' : DComp (fun (c : ctx_base)
+      (f : (a : α_base c) → (h : ∀ b, r_base c b a → Acc (r_base c) b) →
+      (ih : ∀ b hb, motive_base c b (h b hb)) → motive_base c a (Acc.intro a h)) =>
+        fun a : (a : { a : α_base c // ∀ b, r_base c b a → Acc (r_base c) b }) ×'
+          ((b : { b : α_base c // r_base c b a }) → motive_base c b (a.2 b b.2)) =>
+            f a.1 a.1.2 fun b hb => a.2 ⟨b, hb⟩) := by
+    other_dcomp_tac
+  have intro_dcomp_base : DComp intro_base := .unsafeIntro
+  have intro_dcomp : new_type% intro_dcomp_base := intro_comp
+  have_new := this'_base.app intro_dcomp_base
+  clear this' this'_base
   obtain ⟨gi, hgi, hgi'⟩ := this
-  obtain ⟨ga, hga, hga'⟩ := ha
+  obtain ⟨ga, hga, hga'⟩ := a_comp
   obtain ⟨scw, hscw⟩ := Code.exists_code.mp selfCallWith_part
   obtain ⟨th, hth⟩ := Code.exists_code.mp (thing_part scw)
   have hyc := ycomb_part th
   refine ⟨_, .comp hyc (.pair hgi hga), ?_⟩
-  intro n b hn
+  intro b_base b n hn
   obtain ⟨na, hna, hna'⟩ := hga' hn
   obtain ⟨ni, hni, hc⟩ := hgi' hn
   let c := Denumerable.ofNat Code ni
-  rw [encodes_pi_def] at hc
-  clear hga' hgi' hintro
-  specialize t b
-  have (eq := haeq) a := a b
-  dsimp +instances only
-  rw! [← haeq] at t hna' ⊢
+  rw [encoding_pi_def ‹_›] at hc
+  clear hga' hgi' intro_comp intro_dcomp intro_dcomp_base this_base
+  revert hna' hc
+  run_tac
+    let names : Array Lean.Name := #[`t, `a, `intro, `motive, `r, `α]
+    let b_base := mkIdent `b_base
+    let b := mkIdent `b
+    for nm in names do
+      let id := mkIdent nm
+      let bid := mkIdent (nm.appendAfter "_base")
+      let pid := mkIdent (nm.appendAfter "'")
+      let pbid := mkIdent (nm.appendAfter "_base'")
+      evalTactic (← `(tactic| let +generalize $pid : new_type% $bid $b_base := $id $b))
+      evalTactic (← `(tactic| revert $pid))
+      evalTactic (← `(tactic| let +generalize $pbid := $bid $b_base))
+      evalTactic (← `(tactic| revert $pbid))
+  intro α_base' α' r_base' r' motive_base' motive' intro_base' intro' a_base' a' t_base' t' hna' hc
+  clear_value α_base' α' r_base' r' motive_base' motive' intro_base' intro' a_base' a' t_base' t'
+  clear α_base α r_base r motive_base motive intro_base intro a_base a t_base t
   simp only [Part.eq_some_iff.mpr hni, Part.map_eq_map, Part.map_some, Part.eq_some_iff.mpr hna,
     seq_eq_bind_map, Part.bind_eq_bind, Part.bind_some]
-  change ∃ y ∈ _, EncodingRelation.Encodes y (@Acc.rec (α b) (r b) (motive b) (intro b) a t)
-  clear hna haeq
-  induction t generalizing na with | intro a ha ih
+  clear hna hni
+  induction t' generalizing na with | @intro a_base a ha_base ha ih
   have hycomb : ∃ g, (∀ n, (ofNat Code g).eval n = ycomb th (Nat.pair ni n)) ∧
       ycomb th (Nat.pair ni na) = c.eval (Nat.pair na g) := by
     refine ⟨Encodable.encode (scw.curry (Encodable.encode (th.curry ni))), ?_, ?_⟩
@@ -133,69 +195,80 @@ theorem New.Acc.rec.computable.{c, v, u}
       simp [hscw, selfCallWith, ycomb]
     · simp [ycomb, hth, thing, c]
   obtain ⟨g, hg, hg'⟩ := hycomb
-  specialize hc (Nat.pair na g)
-    ⟨⟨a, ha⟩, fun q => @Acc.rec (α b) (r b) (motive b) (intro b) q.1 (ha q.1 q.2)⟩
-  specialize hc ⟨by simpa using hna', ?_⟩
+  specialize @hc ⟨⟨a_base, ha_base⟩,
+    fun q => @Acc.rec α_base' r_base' motive_base' intro_base' q.1 (ha_base q.1 q.2)⟩
+    ⟨⟨a, @ha⟩, fun _ q => New.Acc.rec α' r' motive' intro' q.1 (ha q.1 q.2)⟩ (Nat.pair na g)
+    ⟨by simpa using hna', ?_⟩
   · simp only [Nat.unpair_pair]
-    rw [encodes_pi_def]
-    intro x ⟨y, hy⟩ h
-    obtain ⟨z, hz, hz'⟩ := ih y hy x h
+    rw [encoding_pi_def ‹_›]
+    intro ⟨y_base, hy_base⟩ ⟨y, hy⟩ x h
+    obtain ⟨z, hz, hz'⟩ := ih y hy x h.1
     simp only [hg]
     use z, hz, hz'
-  simpa only [hg', c] using hc-/
+  simpa only [hg', c] using hc
 
-example : DComputable (convert_to_new% fun x : Nat => x) := by
+example : DComputable (new% fun x : Nat => x) := by
   dcomp_tac
 
-attribute [dprim] New.PSigma.fst.computable New.PSigma.snd.computable New.PSigma.mk.computable
-  New.PSigma.fst.primrec New.PSigma.snd.primrec New.PSigma.mk.primrec
+set_option linter.unusedVariables false in
+@[other_dprim]
+lemma Acc.rec.dcomp.{c, v, u}
+    {ctx : Sort c} {α : ctx → Sort u} {r : (c : ctx) → α c → α c → Prop}
+    {motive : (c : ctx) → (a : α c) → Acc (r c) a → Sort v}
+    {intro : ∀ (c : ctx) (a : α c) (h : _) (ih : ∀ b hb, motive _ _ (h b hb)),
+      motive c a (Acc.intro a h)} (intro_comp : DComp intro)
+    {a : (c : ctx) → α c} (a_comp : DComp a) {t : (c : ctx) → Acc (r c) (a c)} :
+    DComp fun c => @Acc.rec (α c) (r c) (motive c) (intro c) (a c) (t c) := .unsafeIntro
+
+lemma New.Acc.rec.dcomp.{c, v, u} : new_type% @Acc.rec.dcomp.{c, v, u} :=
+  fun _ _ _ _ _ _ _ _ _ _ _ hi _ _ _ ha _ _ => New.Acc.rec.computable hi ha
 
 @[dprim]
-theorem New.Unit.unit.computable {ctx_base : Sort u} {ctx : convert_to_new_type% ctx_base} :
-    DComputable (convert_to_new% fun _ : ctx_base => ()) := by
-  refine .const' (x := convert_to_new% ()) ?_
+theorem New.Unit.unit.computable {ctx_base : Sort u} {ctx : new_type% ctx_base} :
+    DComputable (new% fun _ : ctx_base => ()) := by
+  refine .const' (x := new% ()) ?_
   exact ⟨0, .zero⟩
 
-example : DComputable (convert_to_new% fun (x : Nat → Nat) y => x y) := by
+example : DComputable (new% fun (x : Nat → Nat) y => x y) := by
   dcomp_tac
 
-example : DComputable (convert_to_new% fun (x : Nat → Nat) y => x (x y)) := by
+example : DComputable (new% fun (x : Nat → Nat) y => x (x y)) := by
   dcomp_tac
 
-example : DComputable (convert_to_new% fun (x : Nat → (_ : Nat) ×' Nat) y => x (x y).2) := by
+example : DComputable (new% fun (x : Nat → (_ : Nat) ×' Nat) y => x (x y).2) := by
   dcomp_tac
 
 @[dprim]
-theorem New.Nat.zero.computable {ctx_base : Sort u} {ctx : convert_to_new_type% ctx_base} :
-    DComputable (convert_to_new% fun _ : ctx_base => _root_.Nat.zero) := by
-  refine .const' (x := convert_to_new% _root_.Nat.zero) ?_
+theorem _root_.New.Nat.zero.computable {ctx_base : Sort u} {ctx : new_type% ctx_base} :
+    DComputable (new% fun _ : ctx_base => Nat.zero) := by
+  refine .const' (x := new% Nat.zero) ?_
   refine ⟨0, ?_⟩
   rfl
 
 @[dprim]
-theorem New.Nat.succ.computable {ctx_base : Sort u} {ctx : convert_to_new_type% ctx_base}
-    {f_base : ctx_base → ℕ} {f : convert_to_new_type% f_base}
-    (f_comp : DComputable (convert_to_new% f_base)) :
-    DComputable (convert_to_new% fun c => _root_.Nat.succ (f_base c)) := by
-  refine .comp ?_ (f := convert_to_new% _root_.Nat.succ) f_comp
-  refine ⟨_root_.Nat.succ, .succ, ?_⟩
+theorem _root_.New.Nat.succ.computable {ctx_base : Sort u} {ctx : new_type% ctx_base}
+    {f_base : ctx_base → ℕ} {f : new_type% f_base}
+    (f_comp : DComputable (new% f_base)) :
+    DComputable (new% fun c => Nat.succ (f_base c)) := by
+  refine .comp ?_ (f := new% Nat.succ) f_comp
+  refine ⟨Nat.succ, .succ, ?_⟩
   intro a _ _ rfl
   exact ⟨a + 1, by simp, by rfl⟩
 
 @[dprim]
-theorem New.Nat.rec.primrec {ctx_base : Sort u} {ctx : convert_to_new_type% ctx_base}
-    {motive_base : ctx_base → ℕ → Sort v} {motive : convert_to_new_type% motive_base}
+theorem _root_.New.Nat.rec.primrec {ctx_base : Sort u} {ctx : new_type% ctx_base}
+    {motive_base : ctx_base → ℕ → Sort v} {motive : new_type% motive_base}
     {zero_base : (c : ctx_base) → motive_base c .zero}
-    {zero : convert_to_new_type% zero_base}
-    (zero_comp : DPrimrec (convert_to_new% zero_base))
+    {zero : new_type% zero_base}
+    (zero_comp : DPrimrec (new% zero_base))
     {succ_base : (c : ctx_base) → (n : ℕ) → motive_base c n → motive_base c (.succ n)}
-    {succ : convert_to_new_type% succ_base}
-    (succ_comp : DPrimrec (convert_to_new%
+    {succ : new_type% succ_base}
+    (succ_comp : DPrimrec (new%
       fun x : (c : ctx_base) ×' (n : ℕ) ×' motive_base c n => succ_base x.1 x.2.1 x.2.2))
-    {t_base : ctx_base → ℕ} {t : convert_to_new_type% t_base}
-    (t_comp : DPrimrec (convert_to_new% t_base)) :
-    DPrimrec (convert_to_new% fun c =>
-      @_root_.Nat.rec (motive_base c) (zero_base c) (succ_base c) (t_base c)) := by
+    {t_base : ctx_base → ℕ} {t : new_type% t_base}
+    (t_comp : DPrimrec (new% t_base)) :
+    DPrimrec (new% fun c =>
+      @Nat.rec (motive_base c) (zero_base c) (succ_base c) (t_base c)) := by
   obtain ⟨fz, hfz, hfz'⟩ := zero_comp
   obtain ⟨fs, hfs, hfs'⟩ := succ_comp
   obtain ⟨ft, hft, hft'⟩ := t_comp
@@ -208,45 +281,43 @@ theorem New.Nat.rec.primrec {ctx_base : Sort u} {ctx : convert_to_new_type% ctx_
   induction ft nc with
   | zero => exact hfz'
   | succ k ih =>
-    specialize @hfs' ⟨c_base, k, _root_.Nat.rec (zero_base c_base) (succ_base c_base) k⟩
-    specialize @hfs' ⟨c, (), Nat.rec (motive c) (zero c) (succ c) ()⟩
+    specialize @hfs' ⟨c_base, k, Nat.rec (zero_base c_base) (succ_base c_base) k⟩
+    specialize @hfs' ⟨c, (), New.Nat.rec (motive c) (zero c) (succ c) ()⟩
     exact @hfs' (Nat.pair nc (Nat.pair k _))
       ⟨by simpa using hnc, by simp; rfl, by simpa using ih⟩
 
-convert_to_new Nat.recAux
-
 @[dprim]
-theorem New.Nat.rec.computable {ctx_base : Sort u} {ctx : convert_to_new_type% ctx_base}
-    {motive_base : ctx_base → ℕ → Sort v} {motive : convert_to_new_type% motive_base}
+theorem _root_.New.Nat.rec.computable {ctx_base : Sort u} {ctx : new_type% ctx_base}
+    {motive_base : ctx_base → ℕ → Sort v} {motive : new_type% motive_base}
     {zero_base : (c : ctx_base) → motive_base c .zero}
-    {zero : convert_to_new_type% zero_base}
-    (zero_comp : DComputable (convert_to_new% zero_base))
+    {zero : new_type% zero_base}
+    (zero_comp : DComputable (new% zero_base))
     {succ_base : (c : ctx_base) → (n : ℕ) → motive_base c n → motive_base c (.succ n)}
-    {succ : convert_to_new_type% succ_base}
-    (succ_comp : DComputable (convert_to_new% succ_base))
-    {t_base : ctx_base → ℕ} {t : convert_to_new_type% t_base}
-    (t_comp : DComputable (convert_to_new% t_base)) :
-    DComputable (convert_to_new% fun c =>
-      @_root_.Nat.rec (motive_base c) (zero_base c) (succ_base c) (t_base c)) := by
-  have := convert_to_new%
-    show (fun c => @_root_.Nat.rec (fun n => _root_.Unit → motive_base c n) (fun _ => zero_base c)
+    {succ : new_type% succ_base}
+    (succ_comp : DComputable (new% succ_base))
+    {t_base : ctx_base → ℕ} {t : new_type% t_base}
+    (t_comp : DComputable (new% t_base)) :
+    DComputable (new% fun c =>
+      @Nat.rec (motive_base c) (zero_base c) (succ_base c) (t_base c)) := by
+  have := new%
+    show (fun c => @Nat.rec (fun n => Unit → motive_base c n) (fun _ => zero_base c)
           (fun n ih _ => succ_base c n (ih ())) (t_base c) ()) =
-        (fun c => @_root_.Nat.rec (motive_base c) (zero_base c) (succ_base c) (t_base c)) by
+        (fun c => @Nat.rec (motive_base c) (zero_base c) (succ_base c) (t_base c)) by
       funext c; induction t_base c <;> simp_all
   dsimp only at this
-  refine Eq._induct.rec (motive := fun a _ _ => DComputable a) ?_ this
+  refine New.Eq._induct.rec (motive := fun a _ _ => DComputable a) ?_ this
   dsimp only
-  have recComp : DComputable (convert_to_new% fun x :
-      (c : ctx_base) ×' (zero : _root_.Unit → motive_base c 0) ×'
-        (succ : (n : ℕ) → (_root_.Unit → motive_base c n) →
-          _root_.Unit → motive_base c (n.succ)) ×' ℕ =>
-      @_root_.Nat.rec (fun n => _root_.Unit → motive_base x.1 n) x.2.1 x.2.2.1 x.2.2.2) := by
+  have recComp : DComputable (new% fun x :
+      (c : ctx_base) ×' (zero : Unit → motive_base c 0) ×'
+        (succ : (n : ℕ) → (Unit → motive_base c n) →
+          Unit → motive_base c (n.succ)) ×' ℕ =>
+      @Nat.rec (fun n => Unit → motive_base x.1 n) x.2.1 x.2.2.1 x.2.2.2) := by
     refine .of_prim ?_
     dcomp_tac
-  have mk : DComputable (convert_to_new% fun c : ctx_base =>
+  have mk : DComputable (new% fun c : ctx_base =>
       (⟨c, fun _ => zero_base c, fun n ih _ => succ_base c n (ih ()), t_base c⟩ :
-        (c : ctx_base) ×' (zero : _root_.Unit → motive_base c 0) ×'
-          (succ : (n : ℕ) → (_root_.Unit → motive_base c n) →
-            _root_.Unit → motive_base c (n.succ)) ×' ℕ)) := by
+        (c : ctx_base) ×' (zero : Unit → motive_base c 0) ×'
+          (succ : (n : ℕ) → (Unit → motive_base c n) →
+            Unit → motive_base c (n.succ)) ×' ℕ)) := by
     dcomp_tac
-  exact .comp (.app recComp Unit.unit.computable) mk
+  exact .comp (.app recComp New.Unit.unit.computable) mk
