DependentComputability/Tactic/LetNew.lean
@@ -1,0 +1,56 @@
+import DependentComputability.SortExtra
+
+open Lean Meta Parser Elab Term Tactic
+partial def letNewHelper (goalType : Expr) (val : Expr) (baseMap : FVarIdMap Expr) :
+    MonadCacheT ExprStructEq Expr MetaM (Expr × MVarId) := do
+  match val with
+  | .letE nm t v b false =>
+    let newType ← conversionStepNew.visit t baseMap
+    let newValue ← conversionStepNew.visit v baseMap
+    withLetDecl (nm.appendAfter "_base") t v fun var_base => do
+    withLetDecl nm (mkExtraApp newType var_base) newValue fun var => do
+      let (res, mvar) ← letNewHelper goalType (b.instantiate1 var_base)
+        (baseMap.insert var_base.fvarId! var)
+      return (← mkLetFVars #[var_base, var] res, mvar)
+  | .letE nm t v b true =>
+    let newType ← conversionStepNew.visit t baseMap
+    let newValue ← conversionStepNew.visit v baseMap
+    withLocalDeclD (nm.appendAfter "_base") t fun var_base => do
+    withLocalDeclD nm (mkExtraApp newType var_base) fun var => do
+      let (res, mvar) ← letNewHelper goalType (b.instantiate1 var_base)
+        (baseMap.insert var_base.fvarId! var)
+      return (mkApp2 (← mkLambdaFVars #[var_base, var] res) v newValue, mvar)
+  | .lam nm t b bi =>
+    let newType ← conversionStepNew.visit t baseMap
+    withLocalDecl (nm.appendAfter "_base") bi t fun var_base => do
+    withLocalDecl nm bi (mkExtraApp newType var_base) fun var => do
+      let (res, mvar) ← letNewHelper goalType (b.instantiate1 var_base)
+        (baseMap.insert var_base.fvarId! var)
+      return (← mkLambdaFVars #[var_base, var] res, mvar)
+  | .app f a =>
+    if f.getAppFn.isMVar then
+      let mvar ← Meta.mkFreshExprSyntheticOpaqueMVar goalType
+      return (mvar, mvar.mvarId!)
+    let (res, mvar) ← letNewHelper goalType f baseMap
+    return (mkApp2 res a (← conversionStepNew.visit a baseMap), mvar)
+  | .mvar _ =>
+    let mvar ← Meta.mkFreshExprSyntheticOpaqueMVar goalType
+    return (mvar, mvar.mvarId!)
+  | _ => throwError "internal error"
+
+def elabLetNewCore (cfg : TSyntax ``letConfig) (decl : TSyntax ``letDecl)
+    (initConfig : LetConfig := {}) : TacticM Unit := do
+  let goal ← getMainGoal
+  goal.withContext do
+    let mvarIdent : Ident ← `(m)
+    let goalType ← goal.getType
+    let res ← runTermElab do
+      let letTerm ← `(let $cfg:letConfig $decl:letDecl; ?$mvarIdent)
+      elabLetDeclCore letTerm goalType initConfig
+    let res ← instantiateMVars res
+    let (result, newGoal) ← (letNewHelper goalType res (← populateBaseMap)).run
+    goal.assign result
+    replaceMainGoal [newGoal]
+
+elab "let_new" cfg:letConfig decl:letDecl : tactic => elabLetNewCore cfg decl
+elab "have_new" cfg:letConfig decl:letDecl : tactic => elabLetNewCore cfg decl { nondep := true }
