DependentComputability/Tactic/OtherDPrimStep.lean
@@ -1,0 +1,553 @@
+import DependentComputability.SortExtra
+
+inductive DComp {α : Sort u} {β : α → Sort v} (f : (a : α) → β a) : Prop where
+  | unsafeIntro
+
+inductive DPrim {α : Sort u} {β : α → Sort v} (f : (a : α) → β a) : Prop where
+  | unsafeIntro
+
+class Irrel (α : Sort u) : Prop where
+  unsafeIntro ::
+
+def _root_.New.DComp.{u, v} : new_type% @DComp.{u, v} :=
+  fun _ _ _ _ _ f => .mk (fun _ => DComputable f) (TrivialEncoding _) (.trivialEncoding _)
+
+def _root_.New.DPrim.{u, v} : new_type% @DPrim.{u, v} :=
+  fun _ _ _ _ _ f => .mk (fun _ => DPrimrec f) (TrivialEncoding _) (.trivialEncoding _)
+
+def _root_.New.Irrel.{u} : new_type% @Irrel.{u} :=
+  fun _ α => .mk (fun _ => Irrelevant α) (TrivialEncoding _) (.trivialEncoding _)
+
+section
+
+set_option linter.unusedVariables.funArgs false
+
+instance instIrrelProof (p : Prop) : Irrel p := .unsafeIntro
+instance instIrrelSort : Irrel (Sort u) := .unsafeIntro
+instance instIrrelForall {α : Sort u} {β : α → Sort v} [∀ a, Irrel (β a)] :
+    Irrel ((a : α) → β a) := .unsafeIntro
+
+lemma DPrim.id {α : Sort u} : DPrim (fun x : α => x) := .unsafeIntro
+lemma DPrim.comp.{u, v, w} {β : Sort v} {γ : β → Sort w} {f : (b : β) → γ b}
+    (hf : DPrim f) {α : Sort u} {g : α → β} (hg : DPrim g) :
+    DPrim (fun x : α => f (g x)) := .unsafeIntro
+lemma DPrim.compComputable.{u, v, w} {β : Sort v} {γ : β → Sort w} {f : (b : β) → γ b}
+    (hf : DPrim f) {α : Sort u} {g : α → β} (hg : DComp g) :
+    DComp (fun x : α => f (g x)) := .unsafeIntro
+lemma DPrim.irrel {α : Sort u} {β : α → Sort v} [∀ a, Irrel (β a)]
+    {f : (a : α) → β a} : DPrim f := .unsafeIntro
+lemma DPrim.proof {α : Sort u} {β : α → Prop}
+    {f : (a : α) → β a} : DPrim f := .irrel
+lemma DPrim.sort {α : Sort u} {f : (a : α) → Sort v} : DPrim f := .irrel
+lemma DPrim.curry {α : Sort u} {β : α → Sort v} {γ : (a : α) → β a → Sort w}
+    {f : (a : α) → (b : β a) → γ a b} (hf : DComp fun c : PSigma β => f c.1 c.2) :
+    DPrim f := .unsafeIntro
+
+lemma DComp.of_prim {α : Sort u} {β : α → Sort v}
+    {f : (a : α) → β a} (hf : DPrim f) : DComp f := .unsafeIntro
+lemma DComp.id {α : Sort u} : DComp (fun x : α => x) := .of_prim .id
+lemma DComp.comp.{u, v, w} {β : Sort v} {γ : β → Sort w} {f : (b : β) → γ b}
+    (hf : DComp f) {α : Sort u} {g : α → β} (hg : DComp g) :
+    DComp (fun x : α => f (g x)) := .unsafeIntro
+lemma DComp.irrel {α : Sort u} {β : α → Sort v} [∀ a, Irrel (β a)]
+    {f : (a : α) → β a} : DComp f := .unsafeIntro
+lemma DComp.proof {α : Sort u} {β : α → Prop}
+    {f : (a : α) → β a} : DComp f := .irrel
+lemma DComp.sort {α : Sort u} {f : (a : α) → Sort v} : DComp f := .irrel
+lemma DComp.curry {α : Sort u} {β : α → Sort v} {γ : (a : α) → β a → Sort w}
+    {f : (a : α) → (b : β a) → γ a b} (hf : DComp fun c : PSigma β => f c.1 c.2) :
+    DComp f := .of_prim (.curry hf)
+lemma DComp.app.{c, u, v}
+    {α : Sort c} {β : α → Sort u} {γ : (a : α) → β a → Sort v}
+    {f : (a : α) → (b : β a) → γ a b} (hf : DComp f)
+    {g : (a : α) → β a} (hg : DComp g) :
+    DComp (fun x : α => f x (g x)) := .unsafeIntro
+
+lemma _root_.New.instIrrelProof : new_type% @instIrrelProof := @instIrrelevant
+lemma _root_.New.instIrrelSort.{u} : new_type% @instIrrelSort.{u} := @instIrrelevantSort
+lemma _root_.New.instIrrelForall.{u, v} : new_type% @instIrrelForall.{u, v} :=
+  fun _ α _ β _ h => @instIrrelevantForall _ α _ β h
+
+lemma _root_.New.DPrim.id.{u} : new_type% @DPrim.id.{u} := @DPrimrec.id
+lemma _root_.New.DPrim.comp.{u, v, w} : new_type% @DPrim.comp.{u, v, w} :=
+  fun _ _ _ _ _ _ _ hf _ _ _ _ _ hg => .comp hf hg
+lemma _root_.New.DPrim.compComputable.{u, v, w} : new_type% @DPrim.compComputable.{u, v, w} :=
+  fun _ _ _ _ _ _ _ hf _ _ _ _ _ hg => hf.compComputable hg
+lemma _root_.New.DPrim.irrel.{u, v} : new_type% @DPrim.irrel.{u, v} :=
+  fun _ _ _ _ _ h _ _ => @DPrimrec.irrelevant _ _ _ _ h _ _
+lemma _root_.New.DPrim.proof.{u} : new_type% @DPrim.proof.{u} := @DPrimrec.proof
+lemma _root_.New.DPrim.sort.{u, v} : new_type% @DPrim.sort.{u, v} := @DPrimrec.sort
+lemma _root_.New.DPrim.curry.{u, v, w} : new_type% @DPrim.curry.{u, v, w} :=
+  fun _ _ _ _ _ _ _ _ _ hf => .curry hf
+
+lemma _root_.New.DComp.of_prim.{u, v} : new_type% @DComp.of_prim.{u, v} :=
+  fun _ _ _ _ _ _ _ hf => .of_prim hf
+lemma _root_.New.DComp.id.{u} : new_type% @DComp.id.{u} := @DComputable.id
+lemma _root_.New.DComp.comp.{u, v, w} : new_type% @DComp.comp.{u, v, w} :=
+  fun _ _ _ _ _ _ _ hf _ _ _ _ _ hg => .comp hf hg
+lemma _root_.New.DComp.irrel.{u, v} : new_type% @DComp.irrel.{u, v} :=
+  fun _ _ _ _ _ h _ _ => @DComputable.irrelevant _ _ _ _ h _ _
+lemma _root_.New.DComp.proof.{u} : new_type% @DComp.proof.{u} := @DComputable.proof
+lemma _root_.New.DComp.sort.{u, v} : new_type% @DComp.sort.{u, v} := @DComputable.sort
+lemma _root_.New.DComp.curry.{u, v, w} : new_type% @DComp.curry.{u, v, w} :=
+  fun _ _ _ _ _ _ _ _ _ hf => .curry hf
+lemma _root_.New.DComp.app.{u, v, w} : new_type% @DComp.app.{u, v, w} :=
+  fun _ _ _ _ _ _ _ _ _ hf _ _ _ hg => .app hf hg
+
+lemma PSigma.mk.dprim {ctx : Sort u} {α : ctx → Sort v} {β : (c : ctx) → α c → Sort w}
+    {f : (c : ctx) → α c} (hf : DPrim f) {g : (c : ctx) → β c (f c)} (hg : DPrim g) :
+    DPrim (fun c => PSigma.mk (f c) (g c)) := .unsafeIntro
+
+lemma PSigma.fst.dprim {ctx : Sort u} {α : ctx → Sort v} {β : (c : ctx) → α c → Sort w}
+    {f : (c : ctx) → PSigma (β c)} (hf : DPrim f) :
+    DPrim (fun c => (f c).1) := .unsafeIntro
+
+lemma PSigma.snd.dprim {ctx : Sort u} {α : ctx → Sort v} {β : (c : ctx) → α c → Sort w}
+    {f : (c : ctx) → PSigma (β c)} (hf : DPrim f) :
+    DPrim (fun c => (f c).2) := .unsafeIntro
+
+lemma PSigma.mk.dcomp {ctx : Sort u} {α : ctx → Sort v} {β : (c : ctx) → α c → Sort w}
+    {f : (c : ctx) → α c} (hf : DComp f) {g : (c : ctx) → β c (f c)} (hg : DComp g) :
+    DComp (fun c => PSigma.mk (f c) (g c)) := .unsafeIntro
+
+lemma PSigma.fst.dcomp {ctx : Sort u} {α : ctx → Sort v} {β : (c : ctx) → α c → Sort w}
+    {f : (c : ctx) → PSigma (β c)} (hf : DComp f) :
+    DComp (fun c => (f c).1) := .unsafeIntro
+
+lemma PSigma.snd.dcomp {ctx : Sort u} {α : ctx → Sort v} {β : (c : ctx) → α c → Sort w}
+    {f : (c : ctx) → PSigma (β c)} (hf : DComp f) :
+    DComp (fun c => (f c).2) := .unsafeIntro
+
+lemma _root_.New.PSigma.mk.dprim.{u, v, w} : new_type% @PSigma.mk.dprim.{u, v, w} :=
+  fun _ _ _ _ _ _ _ _ _ hf _ _ _ hg => New.PSigma.mk.primrec hf hg
+lemma _root_.New.PSigma.fst.dprim.{u, v, w} : new_type% @PSigma.fst.dprim.{u, v, w} :=
+  fun _ _ _ _ _ _ _ _ _ hf => New.PSigma.fst.primrec hf
+lemma _root_.New.PSigma.snd.dprim.{u, v, w} : new_type% @PSigma.snd.dprim.{u, v, w} :=
+  fun _ _ _ _ _ _ _ _ _ hf => New.PSigma.snd.primrec hf
+lemma _root_.New.PSigma.mk.dcomp.{u, v, w} : new_type% @PSigma.mk.dcomp.{u, v, w} :=
+  fun _ _ _ _ _ _ _ _ _ hf _ _ _ hg => New.PSigma.mk.computable hf hg
+lemma _root_.New.PSigma.fst.dcomp.{u, v, w} : new_type% @PSigma.fst.dcomp.{u, v, w} :=
+  fun _ _ _ _ _ _ _ _ _ hf => New.PSigma.fst.computable hf
+lemma _root_.New.PSigma.snd.dcomp.{u, v, w} : new_type% @PSigma.snd.dcomp.{u, v, w} :=
+  fun _ _ _ _ _ _ _ _ _ hf => New.PSigma.snd.computable hf
+
+end
+
+namespace DPrimrec.Tactic.Other
+
+open Lean Meta Elab Term Tactic Qq
+
+def projToFn (x : Expr) : MetaM Expr := do
+  if let .proj t i e := x then
+    let info := getStructureInfo (← getEnv) t
+    let some name := info.getProjFn? i |
+      throwError "bad projection: field index {i} out of bounds for type {t}"
+    let type ← inferType e
+    let type ← whnfD type
+    type.withApp fun c args => do
+      unless c.isConstOf t do
+        throwError "bad projection: structure type name mismatch"
+      return .app (mkAppN (.const name c.constLevels!) args) e
+  else
+    return x
+
+inductive ParamComputability where
+  | always
+  | prim
+  | computable
+
+structure TheoremInfo where
+  prim : Bool
+  declName : Name
+  thmName : Name
+  paramInfos : Array ParamComputability
+
+structure DPrimTheorems where
+  primTheorems : NameMap TheoremInfo := {}
+  compTheorems : NameMap TheoremInfo := {}
+deriving Inhabited
+
+def DPrimTheorems.add (ths : DPrimTheorems) (th : TheoremInfo) : DPrimTheorems :=
+  if th.prim then
+    { ths with primTheorems := ths.primTheorems.insert th.declName th }
+  else
+    { ths with compTheorems := ths.compTheorems.insert th.declName th }
+
+initialize otherDPrimExt : SimplePersistentEnvExtension TheoremInfo DPrimTheorems ←
+  registerSimplePersistentEnvExtension {
+    addEntryFn := DPrimTheorems.add
+    addImportedFn xss :=
+      xss.foldl (init := {}) fun acc xs => xs.foldl (init := acc)
+        fun acc x => acc.add x
+  }
+
+def mkOtherThmEntry (thm : Name) : MetaM TheoremInfo := do
+  let val ← getConstVal thm
+  forallTelescope val.type fun xs body => do
+    let mkApp3 (.const thing [clvl, rlvl]) ctx α f := body |
+      throwError "invalid `other_dprim` attribute, conclusion is not DPrim or DComp"
+    let prim ← match thing with
+      | ``DPrim => pure true
+      | ``DComp => pure false
+      | _ => throwError "invalid `other_dprim` attribute, conclusion is not DPrim or DComp"
+    let .lam nm _ b bi ← whnfR f |
+      throwError "invalid `other_dprim` attribute, conclusion doesn't have a lambda"
+    b.withApp fun x args => do
+      let .const cnm lvls := x |
+        throwError "invalid `other_dprim` attribute, conclusion must be a const"
+      unless lvls == val.levelParams.tail.map Level.param do
+        throwError "invalid `other_dprim` attribute, bad level parameters"
+      unless ctx == xs[0]! do
+        throwError "expected context parameter {ctx} but found {xs[0]!}"
+      let mut map : Array ParamComputability := #[]
+      let mut j := 1
+      for h : i in *...args.size do
+        let arg := args[i]
+        if h : j < xs.size then
+          let var := xs[j]
+          unless arg.eta == var.app (.bvar 0) do
+            throwError "invalid `other_dprim` attribute, parameter #{i} is \
+              {Expr.lam nm ctx arg bi} and not {var} as expected"
+          if h : j + 1 < xs.size then
+            let x := xs[j + 1]
+            let ty ← inferType x
+            if ty.isAppOf ``DComp then
+              map := map.push .computable
+              j := j + 2
+            else if ty.isAppOf ``DPrim then
+              map := map.push .prim
+              j := j + 2
+            else
+              map := map.push .always
+              j := j + 1
+          else
+            map := map.push .always
+            j := j + 1
+        else
+          throwError "invalid `other_dprim` attribute, parameter #{i} out of range"
+      return {
+        prim
+        declName := cnm
+        thmName := thm
+        paramInfos := map
+      }
+
+initialize
+  registerBuiltinAttribute {
+    name := `other_dprim
+    descr := "Attribute for `other_dcomp_tac`"
+    add nm stx kind := do
+      let entry ← MetaM.run' (mkOtherThmEntry nm)
+      modifyEnv (otherDPrimExt.addEntry · entry)
+  }
+
+def idLemma (prim : Bool) : Name :=
+  if prim then ``DPrim.id else ``DComp.id
+
+def sortLemma (prim : Bool) : Name :=
+  if prim then ``DPrim.sort else ``DComp.sort
+
+def natLitLemma (prim : Bool) : Name :=
+  if prim then `DPrim.natLit else `DComp.natLit
+
+def strLitLemma (prim : Bool) : Name :=
+  if prim then `DPrim.strLit else `DComp.strLit
+
+def mkPred (prim : Bool) {u v : Level} {α : Q(Sort u)} {β : Q($α → Sort v)}
+    (f : Q((a : $α) → $β a)) : Q(Prop) :=
+  if prim then
+    q(DPrim $f)
+  else
+    q(DComp $f)
+
+partial def whnfFast (e : Expr) (zeta : Bool) (argsRev : Array Expr := #[]) : MetaM Expr := do
+  match e with
+  | .app f a => whnfFast f zeta (argsRev.push a)
+  | .proj .. => return argsRev.foldr (fun a f => f.app a) (← projToFn e)
+  | .mdata _ e => whnfFast e zeta argsRev
+  | .lam .. => if argsRev.isEmpty then return e else whnfFast (e.betaRev argsRev) zeta
+  | .letE _ _ v b _ =>
+    if zeta then
+      whnfFast (b.instantiate1 v) zeta argsRev
+    else
+      return argsRev.foldr (fun a f => f.app a) e
+  | _ => return argsRev.foldr (fun a f => f.app a) e
+
+def matchFunctionType (e : Expr) : MetaM (Level × Expr × Level × Expr) := do
+  let fty ← whnfD e
+  let .forallE nm tt bb bi := fty | throwFunctionExpected e
+  withLocalDeclD `x tt fun x => do
+    let bb' := bb.instantiate1 x
+    return (← getLevel tt, tt, ← getLevel bb', .lam nm tt bb bi)
+
+structure LocalThm where
+  value : Expr
+  paramInfos : Array ParamComputability
+
+def LocalThm.instantiate (thm : LocalThm) (univ : Name) (clvl : Level) (ctx : Expr) : Expr :=
+  let repl (lvl : Name) : Option Level := if lvl = univ then clvl else none
+  .app (thm.value.instantiateLevelParamsCore repl) ctx
+
+structure Context where
+  contextUniv : Name
+  localPrimThms : FVarIdMap LocalThm
+  localCompThms : FVarIdMap LocalThm
+  zeta : Bool
+
+abbrev M := ReaderT Context <| ReaderT (FVarIdMap Expr) <| MonadCacheT ExprStructEq Expr MetaM
+
+instance : Inhabited (M α) := ⟨(default : MetaM _)⟩
+
+@[inline]
+def withBasicLocalThm (prim : Bool) {clvl tlvl : Level}
+    {ctx : Q(Sort clvl)} {res_lam : Q($ctx → Sort tlvl)}
+    {val : Q((a : $ctx) → $res_lam a)} (val_comp : Q($(mkPred prim val)))
+    (act : M α) : M α := do
+  withReader newContext act
+where
+  newContext (c : Context) : Context :=
+    have u := Level.param c.contextUniv
+    match prim with
+    | true =>
+      let value1 := q(@DPrim.comp.{u} _ _ _ $val_comp)
+      let value2 := q(@DPrim.compComputable.{u} _ _ _ $val_comp)
+      let thm1 : LocalThm := { value := by exact value1, paramInfos := #[.prim] }
+      let thm2 : LocalThm := { value := by exact value2, paramInfos := #[.computable] }
+      { c with localPrimThms := c.localPrimThms.insert val.fvarId! thm1,
+               localCompThms := c.localCompThms.insert val.fvarId! thm2 }
+    | false =>
+      let value := q(@DComp.comp.{u} _ _ _ $val_comp)
+      let thm : LocalThm := { value := by exact value, paramInfos := #[.computable] }
+      { c with localCompThms := c.localCompThms.insert val.fvarId! thm }
+
+@[inline]
+def isAlwaysZeroQ (lvl : Level) : MaybeLevelDefEq lvl Level.zero :=
+  if lvl.isAlwaysZero then
+    .defEq ⟨⟩
+  else
+    .notDefEq
+
+@[inline]
+def withLetDeclQ [MonadControlT MetaM n] [Monad n]
+    (name : Name) {type : Q(Sort u)} (val : Q($type))
+    (k : (var : Q($type)) → $var =Q $val → n α) : n α :=
+  withLetDecl name type val (fun e => k e ⟨⟩)
+
+@[inline]
+def withHaveDeclQ [MonadControlT MetaM n] [Monad n]
+    (name : Name) {type : Q(Sort u)} (val : Q($type))
+    (k : (var : Q($type)) → n α) : n α :=
+  withLetDecl name type val k (nondep := true)
+
+mutual
+partial def handleUnderApplication (prim : Bool) {clvl rlvl : Level}
+    {ctx : Q(Sort clvl)} {res : Q($ctx → Sort rlvl)} (f : Q((a : $ctx) → $res a)) :
+    M Q($(mkPred prim f)) := do
+  let .lam nm _ b bi := id f | unreachable!
+  let (t', t'lvl, b', b'lvl) ← withLocalDeclQ nm bi q($ctx) fun ctx_var => do
+    let ty ← inferType (b.instantiate1 ctx_var)
+    let .forallE nm' t' b' bi' ← whnf ty |
+      throwError "function expected for type {ty} but we have {b.instantiate1 ctx_var}"
+    let t'lvl ← getLevel t'
+    trace[debug] "under-application: {b.instantiate1 ctx_var} has type {ty} : Sort {t'lvl}"
+    let b'lvl ← withLocalDecl nm' bi' t' (getLevel <| b'.instantiate1 ·)
+    let t'lam := Expr.lam nm ctx (t'.abstract #[ctx_var]) bi
+    let b'lam := Expr.lam nm ctx ((Expr.lam nm' t' b' bi').abstract #[ctx_var]) bi
+    pure (t'lam.abstract #[ctx_var], t'lvl, b'lam, b'lvl)
+  have t' : Q($ctx → Sort t'lvl) := t'
+  have b' : Q((c : $ctx) → $t' c → Sort b'lvl) := b'
+  have : rlvl =QL imax t'lvl b'lvl := ⟨⟩
+  have : $res =Q fun c => (x : $t' c) → $b' c x := ⟨⟩
+  let proof ← solveDPrimGoal false q(fun x : PSigma $t' => $f x.1 x.2)
+  match prim with
+  | true | false => return q(.curry $proof)
+
+-- assumes that `f` is a lambda
+partial def solveDPrimGoal (prim : Bool) {clvl rlvl : Level}
+    {ctx : Q(Sort clvl)} {res : Q($ctx → Sort rlvl)}
+    (f : Q((a : $ctx) → $res a)) :
+    M Q($(mkPred prim f)) := withIncRecDepth do
+  withTraceNode `debug (return m!"{exceptEmoji ·} trying to solve goal{indentExpr f}") do
+  if let .defEq _ := isAlwaysZeroQ rlvl then
+    match prim with
+    | true | false => return q(.proof)
+  let .lam nm _ b bi := id f | unreachable!
+  let b ← whnfFast b (← read).zeta
+  b.withApp fun fn args => do
+  let thm ← match fn with
+    | .sort u =>
+      assert! args.isEmpty
+      return mkApp2 (.const (sortLemma prim) [clvl, u.succ]) ctx f
+    | .forallE .. =>
+      assert! args.isEmpty
+      return ← withLocalDecl nm bi ctx fun ctx_var => do
+        let univ ← getLevel (fn.instantiate1 ctx_var)
+        return mkApp2 (.const (sortLemma prim) [clvl, univ]) ctx f
+    | .lit (.natVal _) =>
+      assert! args.isEmpty
+      return mkApp2 (.const (natLitLemma prim) [clvl]) ctx fn
+    | .lit (.strVal _) =>
+      assert! args.isEmpty
+      return mkApp2 (.const (strLitLemma prim) [clvl]) ctx fn
+    | .lam .. =>
+      assert! args.isEmpty
+      return ← handleUnderApplication prim q($f)
+    | .letE nm' t v b _ =>
+      let tlvl ← withLocalDecl nm bi ctx fun var => getLevel (t.instantiate1 var)
+      have letTyLam : Q($ctx → Sort tlvl) := .lam nm ctx t bi
+      have letTy : Q(Sort imax clvl tlvl) := .forallE nm ctx t bi
+      have : $letTy =Q ∀ c : $ctx, $letTyLam c := ⟨⟩
+      have letVal : Q($letTy) := .lam nm ctx v bi
+      -- add the variable
+      return ← withLetDeclQ nm' q($letVal) fun (var : Q($letTy)) _ => do
+        have b := mkAppN (b.instantiate1 (.app var (.bvar 0))) args
+        have f' : Q((a : $ctx) → $res a) := .lam nm ctx b bi
+        have : $f' =Q $f := ⟨⟩
+        if let .defEq _ := isAlwaysZeroQ tlvl then
+          let res ← solveDPrimGoal prim q($f)
+          return ← mkLetFVars #[var] res
+        let valcomp ← solveDPrimGoal prim q($letVal)
+        have valcomp : Q($(mkPred prim q($var))) := valcomp
+        -- add a computability/primrec proof
+        withHaveDeclQ (nm'.appendAfter "_comp") q($valcomp) fun var_comp => do
+        withBasicLocalThm prim (val := q($var)) q($var_comp) do
+          let res ← solveDPrimGoal prim q($f')
+          mkLetFVars #[var, var, var_comp] (generalizeNondepLet := false) res
+    | .const nm us =>
+      let state := otherDPrimExt.getState (← getEnv)
+      let thms := if prim then state.primTheorems else state.compTheorems
+      let some thm := thms.get? nm |
+        throwError "no {if prim then "primrec" else "computability"} theorem available for {nm}"
+      pure ⟨.const thm.thmName (.param (← read).contextUniv :: us), thm.paramInfos⟩
+    | .fvar var =>
+      let thms ← if prim then pure (← read).localPrimThms else pure (← read).localCompThms
+      let some thm := thms.get? var |
+        throwError "no local {if prim then "primrec" else "computability"} \
+          theorem available for {fn}"
+      pure thm
+    | .bvar idx =>
+      assert! idx == 0
+      pure ⟨.const (idLemma prim) [.param (← read).contextUniv], #[]⟩
+    | .mvar _ => throwError "expression has metavariables"
+    | .proj .. | .app _ _ | .mdata _ _ => unreachable!
+  if args.isEmpty && thm.paramInfos.isEmpty then
+    -- fast path
+    return thm.instantiate (← read).contextUniv clvl ctx
+  if args.size < thm.paramInfos.size then
+    -- under-application
+    return ← handleUnderApplication prim q($f)
+  let mut val := thm.instantiate (← read).contextUniv clvl q($ctx)
+  for arg in args, param in thm.paramInfos do
+    let (argT, arglvl) ← withLocalDecl nm bi ctx fun var => do
+      let argT ← inferType (arg.instantiate1 var)
+      let arglvl ← getLevel argT
+      return (.lam nm ctx (argT.abstract #[var]) bi, arglvl)
+    have argT : Q($ctx → Sort arglvl) := argT
+    have argLambda : Q((c : $ctx) → $argT c) := .lam nm ctx arg bi
+    val := val.app argLambda
+    match param with
+    | .always => continue
+    | .prim =>
+      let .forallE _ (mkApp3 (.const ``DPrim [u, v]) α β g) _ _ ←
+          inferType val | throwError "invalid lemma"
+      let subgoal ← @solveDPrimGoal true u v α β g
+      val := val.app subgoal
+    | .computable =>
+      let subgoal ← solveDPrimGoal false q($argLambda)
+      val := val.app subgoal
+  if args.size = thm.paramInfos.size then
+    return val
+  -- over-application (ensure we are in computable territory)
+  let false := prim |
+    try
+      return ← handleUnderApplication prim q($f)
+    catch _ =>
+      withLocalDecl nm bi ctx fun var => do
+        throwError "invalid over-application in primrec goal: \
+          expected at most {thm.paramInfos.size} arguments but found {args.size} in\
+          {indentExpr <| b.instantiate1 var}"
+  let mut type ←
+    withLocalDeclQ nm bi q($ctx) fun var => do
+      let mut type ← inferType ((mkAppN fn (args.take thm.paramInfos.size)).instantiate1 var)
+      if type.getForallArity < args.size - thm.paramInfos.size then
+        type ← liftM <| forallBoundedTelescope type (some (args.size - thm.paramInfos.size))
+            mkForallFVars
+      return type.abstract #[var]
+  let mut b := mkAppN fn (args.take thm.paramInfos.size)
+  for arg in args[thm.paramInfos.size...*] do
+    let .forallE nm' t' b' bi' := id type | throwError "error"
+    let t'lvl ← withLocalDecl nm bi ctx fun var => getLevel (t'.instantiate1 var)
+    let b'lvl ← withLocalDecl nm bi ctx fun var =>
+      withLocalDecl nm' bi' (t'.instantiate1 var) fun var' =>
+        getLevel (b'.instantiate #[var, var'])
+    have t'lam : Q($ctx → Sort t'lvl) := .lam nm ctx t' bi
+    have b'lam : Q((c : $ctx) → $t'lam c → Sort b'lvl) :=
+      .lam nm ctx (.lam nm' t' b' bi') bi
+    have bLambda : Q((c : $ctx) → (a : $t'lam c) → $b'lam c a) := .lam nm ctx b bi
+    have argLambda : Q((c : $ctx) → $t'lam c) := .lam nm ctx arg bi
+    have val' : Q(DComp $bLambda) := val
+    let argProof ← solveDPrimGoal false q($argLambda)
+    val := q(DComp.app $val' $argProof)
+    type := b'.instantiate1 arg
+    b := b.app arg
+  return val
+
+end
+
+partial def isTriviallyIrrelevant (e : Expr) : MetaM <| Option (Level × Expr) := do
+  if let .sort u := e then
+    return some ⟨u.succ, q(instIrrelSort.{u})⟩
+  else if let .forallE nm t b bi := id e then
+    withLocalDecl nm bi t fun var => do
+      let some ⟨v, irrel⟩ ← isTriviallyIrrelevant (b.instantiate1 var) | return none
+      let ⟨u, t⟩ ← getLevelQ t
+      have blam : Q($t → Sort v) := .lam nm t b bi
+      let _irrel : Q((x : $t) → Irrel ($blam x)) ← mkLambdaFVars #[var] irrel
+      return some ⟨u.imax v, q(@instIrrelForall $t $blam)⟩
+  else
+    return none
+
+elab "other_dcomp_tac" : tactic => do
+  let goal ← getMainGoal
+  goal.withContext do
+  let type ← withReducible <| goal.getType'
+  let mkApp3 (.const nm [clvl, rlvl]) ctx res f := type |
+    throwError "invalid goal for other_dcomp_tac: {type}"
+  let prim ←
+    if nm = ``DComp then pure false
+    else if nm = ``DPrim then pure true
+    else throwError "invalid goal for other_dcomp_tac: {type}"
+  have ctx : Q(Sort clvl) := ctx
+  have res : Q($ctx → Sort rlvl) := res
+  have f : Q((c : $ctx) → $res c) := f
+  let ctxUniv := mkFreshLevelName (← getLevelNames)
+  let mut context := {
+    contextUniv := ctxUniv
+    localPrimThms := {}
+    localCompThms := {}
+    zeta := false
+  }
+  for decl in (← getLCtx) do
+    let type ← whnfR decl.type
+    if let mkApp3 (.const ``DComputable [tlvl, blvl]) t b f@(.fvar _) := type then
+      have t : Q(Sort tlvl) := t
+      have b : Q($t → Sort blvl) := b
+      have f : Q((x : $t) → $b x) := f
+      have e : Q(DComp $f) := decl.toExpr
+      context := withBasicLocalThm.newContext false q($e) context
+    else
+      let .forallE nm t b bi := id type | continue
+      context ← withLocalDecl nm bi t fun var => do
+        let some ⟨v, irrel⟩ ← isTriviallyIrrelevant (b.instantiate1 var) |
+          return context
+        let ⟨u, t⟩ ← getLevelQ t
+        have blam : Q($t → Sort v) := .lam nm t b bi
+        let _irrel : Q((x : $t) → Irrel ($blam x)) ← mkLambdaFVars #[var] irrel
+        have f : Q((a : $t) → $blam a) := decl.toExpr
+        have e : Q(DPrim $f) := q(.irrel)
+        return withBasicLocalThm.newContext true q($e) context
+  let baseMap ← populateBaseMap
+  let res ← (solveDPrimGoal prim q($f)).run context |>.run baseMap |>.run
+  goal.assign res
+
+end DPrimrec.Tactic.Other
